*** empty log message ***

doc-src/TutorialI/Inductive/Star.thy
@@ -1,9 +1,9 @@
 (*<*)theory Star = Main:(*>*)
 
-section{*The transitive and reflexive closure*}
+section{*The reflexive transitive closure*}
 
 text{*
-A perfect example of an inductive definition is the transitive, reflexive
+A perfect example of an inductive definition is the reflexive transitive
 closure of a relation. This concept was already introduced in
 \S\ref{sec:rtrancl}, but it was not shown how it is defined. In fact,
 the operator @{text"^*"} is not defined inductively but via a least
@@ -11,46 +11,52 @@ fixpoint because at that point in the theory hierarchy
 inductive definitions are not yet available. But now they are:
 *}
 
-consts trc :: "('a \<times> 'a)set \<Rightarrow> ('a \<times> 'a)set"  ("_*" [1000] 999)
+consts rtc :: "('a \<times> 'a)set \<Rightarrow> ('a \<times> 'a)set"  ("_*" [1000] 999)
 inductive "r*"
 intros
-trc_refl[intro!]:                        "(x,x) \<in> r*"
-trc_step: "\<lbrakk> (x,y) \<in> r*; (y,z) \<in> r \<rbrakk> \<Longrightarrow> (x,z) \<in> r*"
+rtc_refl[intro!]:                        "(x,x) \<in> r*"
+rtc_step: "\<lbrakk> (x,y) \<in> r*; (y,z) \<in> r \<rbrakk> \<Longrightarrow> (x,z) \<in> r*"
 
 lemma [intro]: "(x,y) : r \<Longrightarrow> (x,y) \<in> r*"
-by(blast intro: trc_step);
+by(blast intro: rtc_step);
 
 lemma step2[rule_format]:
   "(y,z) \<in> r*  \<Longrightarrow> (x,y) \<in> r \<longrightarrow> (x,z) \<in> r*"
-apply(erule trc.induct)
+apply(erule rtc.induct)
  apply(blast);
-apply(blast intro: trc_step);
+apply(blast intro: rtc_step);
 done
 
-lemma trc_trans[rule_format]:
+lemma rtc_trans[rule_format]:
   "(x,y) \<in> r*  \<Longrightarrow> \<forall>z. (y,z) \<in> r* \<longrightarrow> (x,z) \<in> r*"
-apply(erule trc.induct)
+apply(erule rtc.induct)
  apply blast;
 apply(blast intro: step2);
 done
 
-consts trc2 :: "('a \<times> 'a)set \<Rightarrow> ('a \<times> 'a)set"
-inductive "trc2 r"
+consts rtc2 :: "('a \<times> 'a)set \<Rightarrow> ('a \<times> 'a)set"
+inductive "rtc2 r"
 intros
-"(x,y) \<in> r \<Longrightarrow> (x,y) \<in> trc2 r"
-"(x,x) \<in> trc2 r"
-"\<lbrakk> (x,y) \<in> trc2 r; (y,z) \<in> trc2 r \<rbrakk> \<Longrightarrow> (x,z) \<in> trc2 r"
+"(x,y) \<in> r \<Longrightarrow> (x,y) \<in> rtc2 r"
+"(x,x) \<in> rtc2 r"
+"\<lbrakk> (x,y) \<in> rtc2 r; (y,z) \<in> rtc2 r \<rbrakk> \<Longrightarrow> (x,z) \<in> rtc2 r"
 
+text{*
+The equivalence of the two definitions is easily shown by the obvious rule
+inductions:
+*}
 
-lemma "((x,y) \<in> trc2 r) = ((x,y) \<in> r*)"
-apply(rule iffI);
- apply(erule trc2.induct);
-   apply(blast);
+lemma "(x,y) \<in> rtc2 r \<Longrightarrow> (x,y) \<in> r*"
+apply(erule rtc2.induct);
   apply(blast);
- apply(blast intro: trc_trans);
-apply(erule trc.induct);
- apply(blast intro: trc2.intros);
-apply(blast intro: trc2.intros);
+ apply(blast);
+apply(blast intro: rtc_trans);
+done
+
+lemma "(x,y) \<in> r* \<Longrightarrow> (x,y) \<in> rtc2 r"
+apply(erule rtc.induct);
+ apply(blast intro: rtc2.intros);
+apply(blast intro: rtc2.intros);
 done
 
 (*<*)end(*>*)
